@prefix : <https://rs.tdwg.org/bdqffdq/terms/> .
@prefix owl: <http://www.w3.org/2002/07/owl#> .
@prefix rdf: <http://www.w3.org/1999/02/22-rdf-syntax-ns#> .
@prefix xml: <http://www.w3.org/XML/1998/namespace> .
@prefix xsd: <http://www.w3.org/2001/XMLSchema#> .
@prefix rdfs: <http://www.w3.org/2000/01/rdf-schema#> .
@prefix skos: <http://www.w3.org/2004/02/skos/core#> .
@base <https://rs.tdwg.org/bdqffdq/terms/> .

<https://rs.tdwg.org/bdqffdq/terms> rdf:type owl:Ontology ;
                                     rdfs:comment "The classes and object properties found in this ontology are dedicated to fundamental and derived concepts from the Fitness For Use Framework described in the paper by Veiga et al available at: http://journals.plos.org/plosone/article?id=10.1371/journal.pone.0178731" ;
                                     rdfs:label "Biodiversity Data Quality Fittnes for Use Framework" .

#################################################################
#    Annotation properties
#################################################################

###  http://www.w3.org/2004/02/skos/core#definition
skos:definition rdf:type owl:AnnotationProperty .


###  http://www.w3.org/2004/02/skos/core#prefLabel
skos:prefLabel rdf:type owl:AnnotationProperty .


#################################################################
#    Object Properties
#################################################################

###  https://rs.tdwg.org/bdqffdq/terms/amendmentProperty
:amendmentProperty rdf:type owl:ObjectProperty ;
                   rdfs:comment "Sub properties of this type group object properties that apply to amendment concepts such as AmendmentPolicy (DQ Needs), AmendmentMethod (DQ Solutions) and Amendment (DQ Reports)." ;
                   rdfs:label "amendment  Property" ;
                   skos:prefLabel "amendment Property" .


###  https://rs.tdwg.org/bdqffdq/terms/appliesTo
:appliesTo rdf:type owl:ObjectProperty ;
           rdfs:comment "If an Assertion forms the oa:body of an oa:Annotation, the appliesTo DataResource would be the oa:target of the Annotation." ;
           rdfs:label "applies To" ;
           skos:definition "Describes the DataResource about which an Assertion is made." ;
           skos:prefLabel "applies To" .


###  https://rs.tdwg.org/bdqffdq/terms/composedOf
:composedOf rdf:type owl:ObjectProperty ;
            rdfs:comment "Describes the properties from a controlled vocabulary that compose an InformationElement. For example, an InformationElement may be \"composedOf\" properties such as dwc:day, dwc:month and dwc:year." ;
            rdfs:label "composed of" ;
            skos:prefLabel "composed of" .


###  https://rs.tdwg.org/bdqffdq/terms/forAmendment
:forAmendment rdf:type owl:ObjectProperty ;
              rdfs:subPropertyOf :amendmentProperty ;
              rdfs:comment "Use to link AmendmentMethods to Amendments.  Describes the relationship between an Amendment concept in bdqffdq (needs, solutions, reports) and a ContextualizedEnhancement." ;
              rdfs:label "for Amendment" ;
              skos:prefLabel "for Amendment" .


###  https://rs.tdwg.org/bdqffdq/terms/forIssue
:forIssue rdf:type owl:ObjectProperty ;
          rdfs:subPropertyOf :issueProperty ;
          rdfs:domain [ rdf:type owl:Restriction ;
                        owl:onProperty :forIssue ;
                        owl:someValuesFrom :Issue
                      ] ;
          rdfs:comment "Use to link IssueMethods to Issues.  Describes the relationship between a problem concept in bdqffdq (needs, solutions, reports) and a ContextualizedIssue." ;
          rdfs:label "for Issue" ;
          skos:prefLabel "for Issue" .


###  https://rs.tdwg.org/bdqffdq/terms/forMeasure
:forMeasure rdf:type owl:ObjectProperty ;
            rdfs:subPropertyOf :measurementProperty ;
            rdfs:comment "Use to link MeasurementMethods to Measures." ;
            rdfs:label "for Measure" ;
            skos:prefLabel "for Measure" .


###  https://rs.tdwg.org/bdqffdq/terms/hasActedUponInformationElement
:hasActedUponInformationElement rdf:type owl:ObjectProperty ;
                                rdfs:subPropertyOf :hasInformationElement ;
                                rdfs:comment "Provides a relationship between bdqffdq concepts and the information elements that are ActedUpon in a test."@en ;
                                rdfs:label "has Acted Upon Information Element" ;
                                skos:prefLabel "has Acted Upon Information Element" .


###  https://rs.tdwg.org/bdqffdq/terms/hasConsultedInformationElement
:hasConsultedInformationElement rdf:type owl:ObjectProperty ;
                                rdfs:subPropertyOf :hasInformationElement ;
                                rdfs:comment "Provides a relationship between bdqffdq concepts and the information elements that are Consulted, but not ActedUpon in a test."@en ;
                                rdfs:label "has Consulted Information Element" ;
                                skos:prefLabel "has Consulted Information Element" .


###  https://rs.tdwg.org/bdqffdq/terms/hasCriterion
:hasCriterion rdf:type owl:ObjectProperty ;
              rdfs:subPropertyOf :issueProperty ,
                                 :validationProperty ;
              rdfs:domain [ rdf:type owl:Restriction ;
                            owl:onProperty :hasCriterion ;
                            owl:someValuesFrom :Criterion
                          ] ;
              rdfs:comment "Used to link the derived concept of a Validation to the fundamental concept of a Criterion."@en ;
              rdfs:label "has Criterion"@en ;
              skos:prefLabel "has Criterion"@en .


###  https://rs.tdwg.org/bdqffdq/terms/hasDataQualityDimension
:hasDataQualityDimension rdf:type owl:ObjectProperty ;
                         rdfs:subPropertyOf :amendmentProperty ,
                                            :issueProperty ,
                                            :measurementProperty ,
                                            :validationProperty ;
                         rdfs:domain [ rdf:type owl:Restriction ;
                                       owl:onProperty :hasDataQualityDimension ;
                                       owl:someValuesFrom :DataQualityDimension
                                     ] ;
                         rdfs:comment "Used to link a derived concept of a DataQualityNeed (Measure, Validation, Amendment, or Issue) to the fundamental concept of a DataQualityDimension.  For a Measure, the dimension of data quality measured.   For a Validation or Issue, the dimension of data quality assessed.  For an Amendment, the dimension of data quality to be improved.  Under the original formulation of the Framework, only Measures have Dimensions." ;
                         rdfs:label "has Data Quality Dimension"@en ;
                         skos:definition "The DataQualityDimension to which a DataQualityNeed Applies." ;
                         skos:prefLabel "has Data Quality Dimension"@en .


###  https://rs.tdwg.org/bdqffdq/terms/hasEnhancement
:hasEnhancement rdf:type owl:ObjectProperty ;
                rdfs:subPropertyOf :amendmentProperty ;
                rdfs:domain [ rdf:type owl:Restriction ;
                              owl:onProperty :hasEnhancement ;
                              owl:someValuesFrom :Enhancement
                            ] ;
                rdfs:comment "Used to link the derived property of an Amendment to the Fundamental property of an Enhancement." ;
                rdfs:label "has Enhancement" ;
                skos:prefLabel "has Enhancement" .


###  https://rs.tdwg.org/bdqffdq/terms/hasInformationElement
:hasInformationElement rdf:type owl:ObjectProperty ;
                       rdfs:domain [ rdf:type owl:Restriction ;
                                     owl:onProperty :hasInformationElement ;
                                     owl:someValuesFrom :InformationElement
                                   ] ;
                       rdfs:comment "Provides a relationship between bdqffdq concepts and the information elements. For example, ContextualizedCriterion uses this property along with hasResourceType to define a criterion in the context of related information elements." ;
                       rdfs:label "has Information Element" ;
                       skos:prefLabel "has Information Element" .


###  https://rs.tdwg.org/bdqffdq/terms/hasParameter
:hasParameter rdf:type owl:ObjectProperty ;
              rdfs:domain :Parameter ;
              rdfs:comment "Expected to be a relationship between a Specification and a Parameter"@en ;
              rdfs:label "has Parameter"@en ;
              skos:definition "A relationship between a test class and a Parameter"@en ;
              skos:prefLabel "has Parameter"@en .


###  https://rs.tdwg.org/bdqffdq/terms/hasResourceType
:hasResourceType rdf:type owl:ObjectProperty ;
                 rdfs:comment "Provides additional metadata, along with the information elements, that describes the level (SingleRecord or MultiRecord) at which the bdqffdq concept operates. For example, an enhancementInContext with resource type of MultiRecord could be used to define an Amendment that applies at the level of multiple record values." ;
                 rdfs:label "has Resource Type" ;
                 skos:prefLabel "has Resource Type" .


###  https://rs.tdwg.org/bdqffdq/terms/hasResponseResult
:hasResponseResult rdf:type owl:ObjectProperty ;
                   rdfs:subPropertyOf :reportProperty ;
                   rdfs:comment "Used in the DQ Report concept to describe response result objects. For example, values could be bdq:RUN_HAS_RESULT or bdq:INTERNAL_PREREQUISITES_NOT_MET.   If Response.results are not objects, use the datatype property hasResponseResultValue"@en ;
                   rdfs:label "has Response Result" ;
                   skos:prefLabel "has Response Result" .


###  https://rs.tdwg.org/bdqffdq/terms/hasResponseStatus
:hasResponseStatus rdf:type owl:ObjectProperty ;
                   rdfs:subPropertyOf :reportProperty ;
                   rdfs:comment "Used in the DQ Report concept to describe result status. For example, in the case of a Validation result, values could be bdq:COMPLIANT or bdq:NON_COMPLIANT." ;
                   rdfs:label "hase Response Status" ;
                   skos:prefLabel "has Response Status" .


###  https://rs.tdwg.org/bdqffdq/terms/hasSpecification
:hasSpecification rdf:type owl:ObjectProperty ;
                  rdfs:domain [ rdf:type owl:Restriction ;
                                owl:onProperty :hasSpecification ;
                                owl:someValuesFrom :Specification
                              ] ;
                  rdfs:comment "Describes the relationship between a derived bdqffdq concept and the fundamental concept of a Specification (technical description of a test)." ;
                  rdfs:label "has Specification" ;
                  skos:prefLabel "has Specification" .


###  https://rs.tdwg.org/bdqffdq/terms/hasUseCase
:hasUseCase rdf:type owl:ObjectProperty ;
            rdfs:domain :UseCase ;
            rdfs:comment "Used by concepts in the DQ Needs category to describe the relationship between DQ Policies (ValidationPolicy, AmendmentPolicy, MeasurementPolicy) and an instance of the UseCase covered by that policy." ;
            rdfs:label "has Use Case" ;
            skos:prefLabel "has Use Case" .


###  https://rs.tdwg.org/bdqffdq/terms/hasValidation
:hasValidation rdf:type owl:ObjectProperty ;
               rdfs:subPropertyOf :validationProperty ;
               rdfs:domain [ rdf:type owl:Restriction ;
                             owl:onProperty :hasValidation ;
                             owl:someValuesFrom :Validation
                           ] ;
               rdfs:comment "Use to link ValidationPolicies and ValidationMethods to Validations.  Describes the relationship between a validation concept in bdqffdq (needs, solutions, reports) and a contextualizedCriterion."@en ;
               rdfs:label "has Validation"@en ;
               skos:prefLabel "has Validation"@en .


###  https://rs.tdwg.org/bdqffdq/terms/implementedBy
:implementedBy rdf:type owl:ObjectProperty ;
               rdfs:domain [ rdf:type owl:Restriction ;
                             owl:onProperty :implementedBy ;
                             owl:someValuesFrom :Mechanism
                           ] ;
               rdfs:comment "Describes the link between the Implementation concept in bdqffdq and the Mechanism that implements some Specification (also defined in Implementation)." ;
               rdfs:label "implemented By" ;
               skos:prefLabel "implemented By" .


###  https://rs.tdwg.org/bdqffdq/terms/improvedBy
:improvedBy rdf:type owl:ObjectProperty ;
            rdfs:domain [ rdf:type owl:Restriction ;
                          owl:onProperty :improvedBy ;
                          owl:someValuesFrom :Amendment
                        ] ;
            rdfs:comment "Had Domain: Amendment, Range Improvement Target.   Asserting improvement target could be improved by the Amendment.  Object property that describes an enhancement, as part of the ImprovementTarget, that would improve data acted upon by some set of measures or validations.  This can be used to determine which measures and validations are improved upon by a given amendment." ;
            rdfs:label "improved By" ;
            skos:prefLabel "improved By" .


###  https://rs.tdwg.org/bdqffdq/terms/includedInPolicy
:includedInPolicy rdf:type owl:ObjectProperty ;
                  rdfs:label "included in Policy" ;
                  skos:definition "Assserts that a Data Quality Need is part of a Policy" ;
                  skos:prefLabel "included In Policy" .


###  https://rs.tdwg.org/bdqffdq/terms/issueProperty
:issueProperty rdf:type owl:ObjectProperty ;
               rdfs:comment "Category of properties that apply to Issues." ;
               rdfs:label "issue Property" ;
               skos:prefLabel "issue Property" .


###  https://rs.tdwg.org/bdqffdq/terms/measurementProperty
:measurementProperty rdf:type owl:ObjectProperty ;
                     rdfs:comment "Sub properties of this type group object properties that apply to measurement concepts such as MeasurementPolicy (DQ Needs), MeasurementMethod (DQ Solutions) and Measure (DQ Reports)." ;
                     rdfs:label "measurement Property" ;
                     skos:prefLabel "measurement Property" .


###  https://rs.tdwg.org/bdqffdq/terms/producesAssertion
:producesAssertion rdf:type owl:ObjectProperty ;
                   rdfs:comment "Connects Implementations with Assertions" ;
                   rdfs:label "produces Assertion" ;
                   skos:definition "Connects an entity that creates an assertion with the assertion." ;
                   skos:prefLabel "produces Assertion" .


###  https://rs.tdwg.org/bdqffdq/terms/reportProperty
:reportProperty rdf:type owl:ObjectProperty ;
                rdfs:comment "Category of properties used in reports." ;
                rdfs:label "report Property" ;
                skos:prefLabel "report Property" .


###  https://rs.tdwg.org/bdqffdq/terms/targetedIssue
:targetedIssue rdf:type owl:ObjectProperty ;
               rdfs:range [ rdf:type owl:Restriction ;
                            owl:onProperty :targetedIssue ;
                            owl:someValuesFrom :ImprovementTarget
                          ] ;
               rdfs:comment "The issue targeted by some problem via the ImprovementTarget object." ;
               rdfs:label "targeted Issue" ;
               skos:definition "Issue where the data conformance with needs may be improved by accepting proposals from an Amendment via an ImprovementTarget." ;
               skos:prefLabel "targeted Issue" .


###  https://rs.tdwg.org/bdqffdq/terms/targetedMeasure
:targetedMeasure rdf:type owl:ObjectProperty ;
                 rdfs:domain [ rdf:type owl:Restriction ;
                               owl:onProperty :targetedMeasure ;
                               owl:someValuesFrom :Measure
                             ] ;
                 rdfs:comment "Describes the relationship between an improvement target and a Measure.  Was, but dimension is too abstract: The dimension targeted by some enhancement via the ImprovementTarget object."@en ;
                 rdfs:label "targeted Measure"@en ;
                 skos:definition "Measure where the data conformance with needs may be improved by accepting proposals from an Amendment via an ImprovementTarget."@en ;
                 skos:prefLabel "targeted Measure"@en .


###  https://rs.tdwg.org/bdqffdq/terms/targetedValidation
:targetedValidation rdf:type owl:ObjectProperty ;
                    rdfs:subPropertyOf owl:topObjectProperty ;
                    rdfs:domain [ rdf:type owl:Restriction ;
                                  owl:onProperty :targetedValidation ;
                                  owl:someValuesFrom :Validation
                                ] ;
                    rdfs:comment "Relates an improvement target to a Validation.  Was: The criteria targeted by some enhancement via the ImprovementTarget object.  But, too abstract."@en ;
                    rdfs:label "targeted Validatiohn"@en ;
                    skos:definition "Validation where the data conformance with needs may be improved by accepting proposals from an Amendment via an ImprovementTarget."@en ;
                    skos:prefLabel "targeted Validation"@en .


###  https://rs.tdwg.org/bdqffdq/terms/validationProperty
:validationProperty rdf:type owl:ObjectProperty ;
                    rdfs:comment "Sub properties of this type group object properties that apply to validation concepts such as ValidationPolicy (DQ Needs), ValidationMethod (DQ Solutions) and Validation (DQ Reports)." ;
                    rdfs:label "validation Property" ;
                    skos:prefLabel "validation Property" .


#################################################################
#    Data properties
#################################################################

###  https://rs.tdwg.org/bdqffdq/terms/hasAuthoritiesDefaults
:hasAuthoritiesDefaults rdf:type owl:DatatypeProperty ;
                        rdfs:range xsd:string ;
                        rdfs:comment "Details of the bdq:sourceAuthoritiy listed in a Specification, along with Parameters that may be provided to the expected response along with their default values." ;
                        rdfs:label "has Authorities and Defaults"@en ;
                        skos:definition "Text describing source authorities and parameters with their default values to attach to a Specification to further specify the behavior described in the expected response." ;
                        skos:prefLabel "has Authorities and Defaults" .


###  https://rs.tdwg.org/bdqffdq/terms/hasExpectedResponse
:hasExpectedResponse rdf:type owl:DatatypeProperty ;
                     rdfs:range xsd:string ;
                     rdfs:comment "The description of the logic of a test Specification.  An expected response is expected to be a data property of a Specification"@en ;
                     rdfs:label "has Expected Response"@en ;
                     skos:definition "Text describing the logic to be followed by an implementation of a Specification specifying the values of ResponseStatus and ResponseResults that should be produced from the evaluation of input InformationElements." ;
                     skos:prefLabel "has Expected Response"@en .


###  https://rs.tdwg.org/bdqffdq/terms/hasResponseComment
:hasResponseComment rdf:type owl:DatatypeProperty ;
                    rdfs:comment "Intended for consumption by human readers of data qualiy reports to understand why particular assertions were made." ;
                    rdfs:label "has Response Comment" ;
                    skos:definition "Free text describing the assertion made in the response and why that conclusion was reached." ;
                    skos:prefLabel "has Response Comment" .


###  https://rs.tdwg.org/bdqffdq/terms/hasResponseResultValue
:hasResponseResultValue rdf:type owl:DatatypeProperty ;
                        rdfs:range xsd:double ;
                        rdfs:comment "Applies to AmendmentAssertions.   To support bdqcore: tests, is expected to carry a key:value list where the keys are the names of ActedUpon Information Elements, and the values are the proposed new values (filling in or replacing the values of those terms in the input)." ;
                        rdfs:label "has response result value" ;
                        skos:prefLabel "has response result value" .


#################################################################
#    Classes
#################################################################

###  https://rs.tdwg.org/bdqffdq/terms#ResponseQualifier
:ResponseQualifier rdf:type owl:Class ;
                   rdfs:subClassOf :ReportConcept ;
                   rdfs:comment "Intended as an extension point for qualifying information about uncertainty or ambiguity." ;
                   rdfs:label "Response Qualifier" ;
                   skos:definition "A report concept to which additional assertions providing additional information beyond that of ResponseResult from the result of the execution of the Specification of a data quality need are attached." ;
                   skos:prefLabel "Response Qualifier" .


###  https://rs.tdwg.org/bdqffdq/terms/AbstractInformationElement
:AbstractInformationElement rdf:type owl:Class ;
                            rdfs:subClassOf :InformationElement ;
                            rdfs:comment "Information elements such as DATE and DAY are abstract, they could reference any representation of those concepts.  In contrast, dwc:eventDate and dwc:day can be linked to concrete Acted Upon or Consulted information elements." ;
                            rdfs:label "Abstract Information Element" ;
                            skos:definition "An InformationElement described in abstract terms and not linked with one or more concrete terms." ;
                            skos:prefLabel "Abstract Information Element" .


###  https://rs.tdwg.org/bdqffdq/terms/ActedUpon
:ActedUpon rdf:type owl:Class ;
           rdfs:subClassOf :InformationElement ;
           rdfs:comment "An information element to which a Result applies."@en ;
           rdfs:label "Acted Upon"@en ;
           skos:definition "An information element, expressed in concrete terms, about which a data quality need expresses assertions about the data quality in that element." ;
           skos:prefLabel "Acted Upon" .


###  https://rs.tdwg.org/bdqffdq/terms/Amendment
:Amendment rdf:type owl:Class ;
           rdfs:subClassOf :AmendmentConcept ,
                           :DataQualityNeed ;
           rdfs:comment """ContextualizedEnhacement in the original framework.   Describes an instance of the enhancement concept in the context of the associated information elements from some controlled vocabulary (fields ActedUpon or Consulted), and a ResourceType of SingleRecord or MultiRecord.  

Describes a proposal for enhancement of original data, which if accepted, would improve the quality of the data for some use. For example: Recommends valid value for taxon name in a single record.  

Amendments may describe proposed changes to data values, or proposed changes to processes for the production and manipulation of data, for example an Amendment on a SingleRecord may provide criteria for proposing that latitude and longitude are transposed in that record, or a similar Amendment on a MultiRecord may provide critera for proposing that all latitudes and longitudes from some data source have been transposed, and the mapping of data values to transport terms should be changed.  

An Amendment is the data quality needs concept that paralells an AmendmentMethod at the solutions level, and an AmmendmentAssertion at the report level.   

AM = { am | am = < ie, e, rt >, ie ∈ IE, e ∈ E ⋀ rt ∈ RT }"""@en ;
           rdfs:label "Amendment"@en ;
           skos:definition "A data quality need that expresses how proposals may be made to improve the fittnes for use of data." ;
           skos:prefLabel "Amendment"@en .


###  https://rs.tdwg.org/bdqffdq/terms/AmendmentAssertion
:AmendmentAssertion rdf:type owl:Class ;
                    rdfs:subClassOf :AmendmentConcept ,
                                    :Assertion ;
                    rdfs:comment """The Amendment assertion type is a report level concept that describes the results of the execution of of a test that performs an AmendmentMethod following some Specification  to proposes changes based on some Amendment. 

An Amendment concept in bdqffdq is expected to carry a ResponseStatus result that includes a status FILLED_IN, AMENDED, as well as a ResponseResult that asserts proposed changes to values from the original data.

DQA(dr) = {dqa | dqa = < am, s, m, r >, am ∈ AM, s ∈ S, m ∈ M , r ∈ R ⋀ dr ∈ DR}""" ;
                    rdfs:label "Amendment Assertion"@en ;
                    skos:definition "An assertion expressing the result of an implementation evaluating an amendment supporting a particular data quality need to improve a particular data resource." ;
                    skos:prefLabel "Amendment Assertion"@en .


###  https://rs.tdwg.org/bdqffdq/terms/AmendmentConcept
:AmendmentConcept rdf:type owl:Class ;
                  rdfs:label "Amendment Concept"@en ;
                  skos:definition "A term involved in proposals of changes to data or process to improve data quallity to fit expressed data quality needs."@en ;
                  skos:prefLabel "Amendment Concept"@en .


###  https://rs.tdwg.org/bdqffdq/terms/AmendmentMethod
:AmendmentMethod rdf:type owl:Class ;
                 rdfs:subClassOf :AmendmentConcept ,
                                 :DataQualityMethod ;
                 rdfs:comment """The AmendmentMethod in bdqffdq is a DQ Solutions level concept describing the relationship between a Specification (technical description of a test) and an Amendment (an enhancement in the context of resource type (SingleRecord or MultiRecord) and associated information elements).

EM(am) = {s | s ⊂ S ⋀ am ∈ AM}""" ;
                 rdfs:label "Amendment Method"@en ;
                 skos:definition "A data quality solution concept that relates an Amendment to its Specifications." ;
                 skos:prefLabel "Amendment Method"@en .


###  https://rs.tdwg.org/bdqffdq/terms/AmendmentPolicy
:AmendmentPolicy rdf:type owl:Class ;
                 rdfs:subClassOf :AmendmentConcept ,
                                 :Policy ;
                 rdfs:comment """A Data Quality needs level concept that describes how some Amendment relates to a UseCase. This relationship defines which amendments are supported by a given UseCase.

EP(u) = {am | am ⊂ AM ⋀ u ∈ U }""" ;
                 rdfs:label "Amendment Policy"@en ;
                 skos:definition "A need concept that relates a UseCase to a set of supporting Amendments."@en ;
                 skos:prefLabel "Amendment Policy"@en .


###  https://rs.tdwg.org/bdqffdq/terms/Assertion
:Assertion rdf:type owl:Class ;
           rdfs:subClassOf :ReportConcept ;
           rdfs:comment "The Assertion type in bdqffdq is the fundamental concept that makes up a data quality report. Assertion can be any one of four types (represented as subClasses), Measure, Validation, Issue, and Amendement.  The assertion concept consists of a Specification (the technical description of a performed test), a data resource (initial values of input data expressed in terms of some controlled vocabulary), the mechanism (external service, actor, or code that performs the test), and some form of result." ;
           rdfs:label "Assertion"@en ;
           skos:definition "A report concept expressing a statement about data quality assertion following some Specification produced by some implementation pertaining to some data resource." ;
           skos:prefLabel "Assertion"@en .


###  https://rs.tdwg.org/bdqffdq/terms/Consulted
:Consulted rdf:type owl:Class ;
           rdfs:subClassOf :InformationElement ;
           rdfs:comment "An Information Element the content of which is examined to assert a result on one or more other Information Elements"@en ;
           rdfs:label "Consulted"@en ;
           skos:definition "An information element, expressed in concrete terms, about which a data quality need examines in order to expresses assertions about the data quality in another Information Element." ;
           skos:prefLabel "Acted Upon" .


###  https://rs.tdwg.org/bdqffdq/terms/Criterion
:Criterion rdf:type owl:Class ;
           rdfs:subClassOf :FundamentalConcept ,
                           :NeedConcept ;
           rdfs:comment "General statement, for example: In a controlled vocabulary.  Composed with both Validations and Issues."@en ;
           rdfs:label "Criterion"@en ;
           skos:definition "Rule against which data are evaluated for conformance to quality criteria."@en ;
           skos:prefLabel "Criterion"@en .


###  https://rs.tdwg.org/bdqffdq/terms/DataQualityDimension
:DataQualityDimension rdf:type owl:Class ;
                      rdfs:subClassOf :FundamentalConcept ,
                                      :NeedConcept ;
                      rdfs:comment "Describes the aspect of data quality (accuracy, precision, completeness, etc.) that a test examines. For example, [precision] in [coordinate precision of single records].  In the original framework only related to Measures, here may be related to any DataQualityNeed."@en ;
                      rdfs:label "Data Quality Dimension"@en ;
                      skos:definition "An aspect of data quality."@en ;
                      skos:prefLabel "Data Quality Dimension" .


###  https://rs.tdwg.org/bdqffdq/terms/DataQualityMethod
:DataQualityMethod rdf:type owl:Class ;
                   rdfs:subClassOf :SolutionsConcept ;
                   rdfs:comment "DataQualityMethods are associative entities that allow Specifications or data quality tests to be reused by supporting a many to many relationship between the two." ;
                   rdfs:label "Data Quality Method"@en ;
                   skos:definition "A solutions concept that relates a data quality need to a Specification." ;
                   skos:prefLabel "Data Quality Method"@en .


###  https://rs.tdwg.org/bdqffdq/terms/DataQualityNeed
:DataQualityNeed rdf:type owl:Class ;
                 rdfs:subClassOf :NeedConcept ;
                 rdfs:comment "Subtypes of DataQualityNeed are the Test Types.  Data Quality Need appoximates the informal concept of Test as used in BDQ Core." ;
                 rdfs:label "Data Quality Need"@en ;
                 skos:definition "A data quality need concept that expresses what assertions may be made about data with respect to fitness for use." ;
                 skos:prefLabel "Data Quality Need"@en .


###  https://rs.tdwg.org/bdqffdq/terms/DataQualityProfile
:DataQualityProfile rdf:type owl:Class ;
                    rdfs:subClassOf :NeedConcept ;
                    rdfs:comment """Profile in bdqffdq is a data quality Needs level concept describing the UseCases that make up some data quality operation such as the behavior of a single actor or workflow producing the relevant assertions.  

DQP (u) = {dqp | dqp = mp(u) ⋃ vp(u) ⋃ ep(u), mp ∈ MP , vp ∈ VP , ep ∈ EP ⋀ u ∈ U }""" ;
                    rdfs:label "Data Quality Profile"@en ;
                    skos:definition "A needs concept expressing the composition of Policies to satisfy a UseCase." ;
                    skos:prefLabel "Data Quality Profile"@en .


###  https://rs.tdwg.org/bdqffdq/terms/DataQualityReport
:DataQualityReport rdf:type owl:Class ;
                   rdfs:subClassOf :ReportConcept ;
                   rdfs:comment "The DataQualityReport concept consists of a set of assertions (MeasureAssertions, ValidationAssertions, IssueAssertions and AmendmentAssertions) that represent the output of a workflow/actor run.  These assertions form an account of the fitness for use of a tested data set for a specified use, as produced by a Mechanism."@en ;
                   rdfs:label "Data Quality Report"@en ;
                   skos:definition "A report concept comprising a set of data quality assertions." ;
                   skos:prefLabel "Data Quality Report"@en .


###  https://rs.tdwg.org/bdqffdq/terms/DataResource
:DataResource rdf:type owl:Class ;
              rdfs:subClassOf :ReportConcept ;
              rdfs:comment """Describes a data resource containing terms from a controlled vocabulary such as (dwc) that can be related to information elements and represents the original values of the data operated on by an assertion test (i.e. an instance of dwc:Occurrence).  Ideally, DataResources have persistent GUIDs.

A data resource could be the oa:target of a oa:Annotation of which an Assertion is the oa:body.

DR = { dr | dr = < id, rt, v >, id ∈ I D, rt ∈ RT , (rt = sr ⋁ rt = ds) ⋀ v ∈ V }""" ;
              rdfs:label "Data Resource"@en ;
              skos:definition "A thing to whch a data quality assertion applies." ;
              skos:prefLabel "Data Resource"@en .


###  https://rs.tdwg.org/bdqffdq/terms/Enhancement
:Enhancement rdf:type owl:Class ;
             rdfs:subClassOf :AmendmentConcept ,
                             :FundamentalConcept ,
                             :NeedConcept ;
             rdfs:comment "General statement, for example: Recommend replacement value from a controlled vocabulary"@en ;
             rdfs:label "Enhancement"@en ;
             skos:definition "Description of a means by which data could be improved."@en ;
             skos:prefLabel "Enhancement"@en .


###  https://rs.tdwg.org/bdqffdq/terms/FundamentalConcept
:FundamentalConcept rdf:type owl:Class ;
                    rdfs:comment "Contrast with derived concepts, which are compositions of two or more fundamental concepts.  See Veiga et al., 2017.   Derived concepts can be organized by test type into Amendment Concept, Validation Concept, Measurement concept or Issue concept.  Derived concepts can also be organized by framework layer into Needs Concept, Solutions Concept, and Report Concept." ;
                    rdfs:label "Fundamental Concept"@en ;
                    skos:definition "Category of fitness for use concepts that are not derived by composition with other concepts."@en ;
                    skos:prefLabel "Fundamental Concept"@en .


###  https://rs.tdwg.org/bdqffdq/terms/Implementation
:Implementation rdf:type owl:Class ;
                rdfs:subClassOf :SolutionsConcept ;
                rdfs:comment """The bdqffdq derived concept of an Implementation describes the relationship between a Specification (technical description of a test) and the mechanism that implements it.

I (s) = {m | m ⊂ M ⋀ s ∈ S}""" ;
                rdfs:label "Implementation"@en ;
                skos:definition "A solutions concept that describes the portion of a Mechanism that carries out the proccess described in a particular Specification." ;
                skos:prefLabel "Implementation"@en .


###  https://rs.tdwg.org/bdqffdq/terms/ImprovementTarget
:ImprovementTarget rdf:type owl:Class ;
                   rdfs:subClassOf :NeedConcept ;
                   rdfs:comment """The ImprovementTarget concept in bdqffdq describes which measures, issues, and validations are improved by some amendment. ImprovementTarget includes relationships between an Amendment and one or more Validations or Measures.

IT(am) = {me ⋃ va | me ∈ ME, va ∈ VA ⋀ am ∈ AM}"""@en ;
                   rdfs:label "Improvement Target"@en ;
                   skos:definition "A specific data quality need for which a specific Amendment is intended to improve." ;
                   skos:prefLabel "Improvement Target"@en .


###  https://rs.tdwg.org/bdqffdq/terms/InformationElement
:InformationElement rdf:type owl:Class ;
                    rdfs:subClassOf :FundamentalConcept ;
                    rdfs:comment "An information element identifies a portion of data to which a test pertains.  The information element in bdqffdq can be represented as a single or composite element that consists of one or more terms from a controlled vocabulary (fields actedUpon or consulted by an assertion test) that identifies concepts in data relevant to a UseCase.  An abstraction or a concrete term that represents relevant content (e.g., coordinates; dwc.decimalLatitude, dwc:decimalLongitude)."@en ;
                    rdfs:label "Information Element"@en ;
                    skos:definition "A portion of data with which a Data Quality Need is concerned." ;
                    skos:prefLabel "Information Element"@en .


###  https://rs.tdwg.org/bdqffdq/terms/Issue
:Issue rdf:type owl:Class ;
       rdfs:subClassOf :DataQualityNeed ,
                       :IssueConcept ;
       rdfs:comment """Added to the original framework.  Inverse of Contextualized Criterion in the original framework.  Describes an instance of the issue concept in terms of the associated information elements from some controlled vocabulary (fields actedUpon or consulted), and a resource type of SingleRecord or MultiRecord.  Describes criteria by which data which lack quality for some purpose may be identified.  An issue is phrased in a negative sense, and approximates an inverse of a Validation.  An Issue identifies data that lack or may lack quality.  An Issue may flag a POTENTIAL_ISSUE that would need further review to determine if the data have quality for some purpose,  If the conditions described by an issue are identified by a test, the Problem Assertion result will be either IS_ISSUE or POTENTIAL_ISSUE, if no issue is found with the data the result will be NOT_ISSUE.  NOT_ISSUE, unlike COMPLIANT for a Validation, does not assert that data are fit for some purpose.    An Issue is the data quality needs concept that paralells a IssueMethod at the solutions level, and a IssueAssertion at the report level.   

IS = { is | is = < ie, c, rt >, ie ∈ IE, c ∈ ∁C ⋀ rt ∈ RT }"""@en ;
       rdfs:label "Issue"@en ;
       skos:definition "A data quality need that expresses how quality problems may be identified in data." ;
       skos:prefLabel "Issue"@en .


###  https://rs.tdwg.org/bdqffdq/terms/IssueAssertion
:IssueAssertion rdf:type owl:Class ;
                rdfs:subClassOf :Assertion ,
                                :IssueConcept ;
                rdfs:comment """The data quality report concept describing a the result of a test in the negative, that is  identifying the potential absence of data quality. 

If a problem was found the ResponseResult is expected to carry a a value of IS_ISSUE, if a potential problem was found that needs human review the ResponseResult is expected to be of POTENTIAL_ISSUE, otherwise if the ResponseStatus is RUN_HAS_RESULT,  the ResponseResult is expected to be NOT_ISSUE.""" ;
                rdfs:label "Issue Assertion"@en ;
                skos:definition "An assertion expressing the result of an implementation evaluating an issue for a particular data quality need in a particular data resource." ;
                skos:prefLabel "Issue Assertion"@en .


###  https://rs.tdwg.org/bdqffdq/terms/IssueConcept
:IssueConcept rdf:type owl:Class ;
              rdfs:comment "Issue terms are expressed in a negative sense, they identify data that do not or may not conform to quality needs."@en ;
              rdfs:label "Issue Concept"@en ;
              skos:definition "A term involved in flagging problems or potential problems in assessment of data quality that would or might prevent the data from meeting expressed data quality needs."@en ;
              skos:prefLabel "Issue Concept"@en .


###  https://rs.tdwg.org/bdqffdq/terms/IssueMethod
:IssueMethod rdf:type owl:Class ;
             rdfs:subClassOf :DataQualityMethod ,
                             :IssueConcept ;
             rdfs:comment "The IssueMethod in bdqffdq is a data quality Solutions level concept describing the relationship between a Specification (technical description of a test) and an Issue (a Criterion in the context of resource type (SingleRecord or MultiRecord) and associated information elements)." ;
             rdfs:label "Issue Method"@en ;
             skos:definition "A data quality solution concept that relates an Issue to its Specifications." ;
             skos:prefLabel "Issue Method"@en .


###  https://rs.tdwg.org/bdqffdq/terms/IssuePolicy
:IssuePolicy rdf:type owl:Class ;
             rdfs:subClassOf :IssueConcept ,
                             :Policy ;
             rdfs:comment "The ProblemPolicy in bdqffdq is a data quality Needs level concept that describes how some contextualizedIssue relates to a UseCase. This relationship defines which problems are supported by a given UseCase." ;
             rdfs:label "Issue Policy"@en ;
             skos:definition "A need concept that relates a UseCase to a set of supporting Issues." ;
             skos:prefLabel "Issue Policy"@en .


###  https://rs.tdwg.org/bdqffdq/terms/Measure
:Measure rdf:type owl:Class ;
         rdfs:subClassOf :DataQualityNeed ,
                         :MeaurementConcept ;
         rdfs:comment """Contextualized Dimension in the original framework  Describes an instance of the measure concept in terms of the associated information elements from some controlled vocabulary (fields ActedUpon or Consulted), and a ResourceType of SingleRecord or MultiRecord. 

Describes the criteria for measuring an aspect of data quality related to some data quality need.   May be criteria for determining that data are COMPLETE or NOT_COMPLETE, or may be criteria for asserting a numeric measurement.  COMPLETE or NOT_COMPLETE measures are fundamental to data quality control, as set of data are filtered to the subset of data that have quality for some need if all records are COMPLETE for all pertenent Measures. 

A Measure is the data quality needs concept that paralells a MeasurementMethod at the solutions level, and a MeasurementAssertion at the report level.

ME = { me | me =< ie, d, rt >, ie ∈ IE, d ∈ D ⋀ rt ∈ RT }
also acceptable measure
AM(me) = {va | me ∈ C D ⋀ va ⊂ C C}"""@en ;
         rdfs:label "Measure"@en ;
         skos:definition "A data quality need that expresses how the fitness of data for some use may be measured." ;
         skos:prefLabel "Measure"@en .


###  https://rs.tdwg.org/bdqffdq/terms/MeasurementAssertion
:MeasurementAssertion rdf:type owl:Class ;
                      rdfs:subClassOf :Assertion ,
                                      :MeaurementConcept ;
                      rdfs:comment """The MeasurementAssertion is a report level concept that describes the results of the execution of of a test that performs a MeasurementMethod according following some Specification  to assess some data quality Measurement. 

In bdqffdq, the MeasurementAssertion is expected to carry a ResponseResult of COMPLETE or NOT_COMPLETE or a numeric measured value value (e.g. a measure of dwc:eventDate duration in seconds).

DQM(dr) = {dqm | dqm =< me, s, m, r >, me ∈ ME, s ∈ S, m ∈ M , r ∈ R ⋀ dr ∈ DR}""" ;
                      rdfs:label "Measurement Assertion"@en ;
                      skos:definition "An assertion expressing the result of an implementation measuring a particular data quality need in a particular data resource." ;
                      skos:prefLabel "Measurement Assertion"@en .


###  https://rs.tdwg.org/bdqffdq/terms/MeasurementMethod
:MeasurementMethod rdf:type owl:Class ;
                   rdfs:subClassOf :DataQualityMethod ,
                                   :MeaurementConcept ;
                   rdfs:comment """The MeasurementMethod in bdqffdq is a data quality Solutions level concept describing the relationship between a Specification (technical description of a test) and a Measurement (a dimension in the context of resource type (SingleRecord or MultiRecord) and associated information elements).

MM(me) = {s | s ⊂ S ⋀ me ∈ ME}""" ;
                   rdfs:label "Measurement Method"@en ;
                   skos:definition "A data quality solution concept that relates a Measure to its Specifications." ;
                   skos:prefLabel "Measurement Method"@en .


###  https://rs.tdwg.org/bdqffdq/terms/MeasurementPolicy
:MeasurementPolicy rdf:type owl:Class ;
                   rdfs:subClassOf :MeaurementConcept ,
                                   :Policy ;
                   rdfs:comment """The MeasurementPolicy in bdqffdq is a data quality Needs level concept that describes how some Measurement relates to a UseCase. This relationship defines which measures are supported by a given UseCase.

MP(u) = {me | me ⊂ ME ⋀ u ∈ U }""" ;
                   rdfs:label "Measurement Policy"@en ;
                   skos:definition "A need concept that relates a UseCase to a set of supporting Measures." ;
                   skos:prefLabel "Measurement Policy"@en .


###  https://rs.tdwg.org/bdqffdq/terms/MeaurementConcept
:MeaurementConcept rdf:type owl:Class ;
                   rdfs:label "Measurement Concept"@en ;
                   skos:definition "A term involved in measurement of data quality with regards to expressed data quality needs."@en ;
                   skos:prefLabel "Measurement Concept"@en .


###  https://rs.tdwg.org/bdqffdq/terms/Mechanism
:Mechanism rdf:type owl:Class ;
           rdfs:subClassOf :FundamentalConcept ,
                           :SolutionsConcept ;
           rdfs:comment """Mechanisms may produce data quality reports as products.    

The bdqffdq concept of mechanism describes the entity that performs an assertion test (code, external service, actor, etc.). Tied to a Specification via the concept of an Implementation.""" ;
           rdfs:label "Mechanism"@en ;
           skos:definition "An entity that can execute data quality methods."@en ;
           skos:prefLabel "Mechanism"@en .


###  https://rs.tdwg.org/bdqffdq/terms/NeedConcept
:NeedConcept rdf:type owl:Class ;
             rdfs:comment "Category of concepts forming the Needs layer of the fitness for use framework." ;
             rdfs:label "Need Concept"@en ;
             skos:definition "A concept that expresses an aspect of a data quality need."@en ;
             skos:prefLabel "Need Concept"@en .


###  https://rs.tdwg.org/bdqffdq/terms/Parameter
:Parameter rdf:type owl:Class ;
           rdfs:subClassOf :SolutionsConcept ;
           rdfs:comment "An extension to the original fittness for use framework as described in Veiga et al., 2017." ;
           rdfs:label "Parameter"@en ;
           skos:definition "A value that, when provided to a test Specification changes the behavior of the test in a defined manner."@en ;
           skos:prefLabel "Parameter"@en .


###  https://rs.tdwg.org/bdqffdq/terms/Policy
:Policy rdf:type owl:Class ;
        rdfs:subClassOf :NeedConcept ;
        rdfs:comment "Composition of data quality Needs into UseCases" ;
        rdfs:label "Policy" ;
        skos:definition "The set of data quality Needs for a UseCase" ;
        skos:prefLabel "Policy" .


###  https://rs.tdwg.org/bdqffdq/terms/ReportConcept
:ReportConcept rdf:type owl:Class ;
               rdfs:comment "Category of concepts forming the Report layer of the fitness for use framework."@en ;
               rdfs:label "Report Concept" ;
               skos:definition "A concept concerning data quality expressed in a data quality report." ;
               skos:prefLabel "Report Concept"@en .


###  https://rs.tdwg.org/bdqffdq/terms/ResourceType
:ResourceType rdf:type owl:Class ;
              rdfs:subClassOf :FundamentalConcept ;
              rdfs:comment "In bdqffdq the concept of ResourceType has instances for SingleRecord or MultiRecord" ;
              rdfs:label "Resource Type"@en ;
              skos:definition "Category of things that are data objects about which data quality assertions may be made." ;
              skos:prefLabel "Resource Type"@en .


###  https://rs.tdwg.org/bdqffdq/terms/ResponseResult
:ResponseResult rdf:type owl:Class ;
                rdfs:subClassOf :ReportConcept ;
                rdfs:comment """For Validations, response results may be COMPLIANT, or NOT_COMPLIANT.  For Measures, response result objects may be COMPLETE or NOT_COMPLETE.  For Issues, Response results may be IS_ISSUE, POTENTIAL_ISSUE, or NOT_ISSUE.  See the bdq: vocabulary.  Measures may also use a numeric data property.  Amendments assert a string data property.

The report ResponseResult in bdqffdq is represented as a value or a result object for MeasureAsssertions, just a result object for ValidationAssertions and values for changes propsed in AmendmentAssertions.""" ;
                rdfs:label "Response.result"@en ;
                skos:definition "A report concept to which a controlled vocabulary assertions about the result of the execution of the Specification of a data quality need are attached." ;
                skos:prefLabel "Response.result"@en .


###  https://rs.tdwg.org/bdqffdq/terms/ResponseStatus
:ResponseStatus rdf:type owl:Class ;
                rdfs:subClassOf :ReportConcept ;
                rdfs:comment "The ResponseStatus is metadata, indicating if data should be present in a ResponseResult.   Any assertion may have the values INTERNAL_PREREQUISITES_NOT_MET of EXTERNAL_PREREQUISITES_NOT_MET, indicating that no value would be present in the accompanying ResponseResult.  Other values depend on the Assertion type.  Thes would be RUN_HAS_RESULT for a Validation, Measure, or Isssue, and, FILLED_IN, AMENDED, or NOT_AMENDED for an Amendment.  Additional metadata qualifying the assertion in a ReqponseResult, such as statements of uncertainy or ambiguity may be placed in the ResponseQualifier" ;
                rdfs:label "Response.status"@en ;
                skos:definition "A report concept expressing controlled vocabulary values about the exit state of an execution process of a data quality Specification by an implementation." ;
                skos:prefLabel "Response.status"@en .


###  https://rs.tdwg.org/bdqffdq/terms/SolutionsConcept
:SolutionsConcept rdf:type owl:Class ;
                  rdfs:comment "Category of concepts forming the Solutions layer of the fitness for use framework.  Solutions are tools that evaluate data against needs and express conclusions in data quality reports."@en ;
                  rdfs:label "Solutions Concept"@en ;
                  skos:definition "A concept that expresses an aspect of a data quality solution." ;
                  skos:prefLabel "Solutions Concept"@en .


###  https://rs.tdwg.org/bdqffdq/terms/Specification
:Specification rdf:type owl:Class ;
               rdfs:subClassOf :FundamentalConcept ,
                               :SolutionsConcept ;
               rdfs:comment "A Specification is a technical desription of an assertion test.  A Specification is expected to have the following properies:  (1) Expected Response, (2) Authorities and Parameters."@en ;
               rdfs:label "Specification"@en ;
               skos:definition "A specific statement about how to evaluate a data quality need."@en ;
               skos:prefLabel "Specification"@en .


###  https://rs.tdwg.org/bdqffdq/terms/UseCase
:UseCase rdf:type owl:Class ;
         rdfs:subClassOf :FundamentalConcept ,
                         :NeedConcept ;
         rdfs:comment "The UseCase concept in bdqffdq describes some data quality control UseCase. The Amendment, Measurement and Validation policies that make up a UseCase define which assertions cover a given UseCase.  An example of a UseCase could be \"Check for internal consistency of dates\", with validation policies for checking consistency between atomic date fields and an Amendment such as \"eventDate filled in from verbatim\".  UseCases in bdqffdq are not the same as UseCases in the software engineering sense, but are similar bdqffdq formal statements derived from analyis of user stories." ;
         rdfs:label "Use Case"@en ;
         skos:definition "A needs concept expressing a purpose to which data are put for which the data must have quality for the result to have meaning and reliability." ;
         skos:prefLabel "Use Case"@en .


###  https://rs.tdwg.org/bdqffdq/terms/Validation
:Validation rdf:type owl:Class ;
            rdfs:subClassOf :DataQualityNeed ,
                            :ValidationConcept ;
            rdfs:comment """ContextualizedCriterion in the original framework.  Describes the criteria for determining compliance of data to fill some data quality need.  A description of a criterion applied to an information element for some resource type.   Describes an instance of the criterion concept in terms of the associated information elements from some controlled vocabulary (fields actedUpon or consulted), and a resource type of SingleRecord or MultiRecord.  

Validations are phrased in a positive sense, they identify data which has quality for some need.  For example: The value of basisOfRecord of single records must be in the controlled vocabulary.   

A Validation is the data quality needs concept that paralells a ValidationMethod at the solutions level, and a ValidationAssertion at the report level.  ValidationAssertions may specify a result that is COMPLIANT, where the data has quality, or NOT_COMPLIANT, where the data lacks quality for some use.  

VA = { va | va = < ie, c, rt >, ie ∈ IE, c ∈ C ⋀ rt ∈ RT }"""@en ;
            rdfs:label "Validation"@en ;
            skos:definition "A data quality need that expreses how data may be evaluated for fitness for use."@en ;
            skos:prefLabel "Validation"@en .


###  https://rs.tdwg.org/bdqffdq/terms/ValidationAssertion
:ValidationAssertion rdf:type owl:Class ;
                     rdfs:subClassOf :Assertion ,
                                     :ValidationConcept ;
                     rdfs:comment """The ValidationAssertion is a report level concept that describes the results of the execution of of a test that performs a ValidationMethod according following some Specification  to assess the validity of some data with respect to the Criteria of some Validation. 

The ValidationAssertion concept in bdqffdq is expected to carry a a ResponseResult of COMPLIANT or NON_COMPLIANT.

DQV(dr) = {dqv | dqv = < va, s, m, r >, va ∈ VA, s ∈ S, m ∈ M , r ∈ R ⋀ dr ∈ DR}""" ;
                     rdfs:label "Validation Assertion"@en ;
                     skos:definition "An assertion expressing the result of an implementation validating compliance with a a particular data quality need in a particular data resource." ;
                     skos:prefLabel "Validation Assertion"@en .


###  https://rs.tdwg.org/bdqffdq/terms/ValidationConcept
:ValidationConcept rdf:type owl:Class ;
                   rdfs:comment "Validation terms are expressed in a positive sense, they identify data that conform to needs."@en ;
                   rdfs:label "Validation Concept"@en ;
                   skos:definition "A term involved in statements about the conformance of data to expressed quality needs."@en ;
                   skos:prefLabel "Validation Concept"@en .


###  https://rs.tdwg.org/bdqffdq/terms/ValidationMethod
:ValidationMethod rdf:type owl:Class ;
                  rdfs:subClassOf :DataQualityMethod ,
                                  :ValidationConcept ;
                  rdfs:comment """The ValidationMethod in bdqffdq is a data quality Solutions level concept describing the relationship between a Specification (technical description of a test) and a Validation (a Criterion in the context of resource type (SingleRecord or MultiRecord) and associated information elements).

VM(va) = {s | s ⊂ S ⋀ va ∈ VA}""" ;
                  rdfs:label "Validation Method"@en ;
                  skos:definition "A data quality solution concept that relates an Validation to its Specifications." ;
                  skos:prefLabel "Validation Method"@en .


###  https://rs.tdwg.org/bdqffdq/terms/ValidationPolicy
:ValidationPolicy rdf:type owl:Class ;
                  rdfs:subClassOf :Policy ,
                                  :ValidationConcept ;
                  rdfs:comment """The ValidationPolicy in bdqffdq is a data quality Needs level concept that describes how some Validation relates to a UseCase. This relationship defines which Validations are needed to identify quality in a given UseCase.

VP (u) = {va | va ⊂ VA ⋀ u ∈ U }""" ;
                  rdfs:label "Validation Policy"@en ;
                  skos:definition "A need concept that relates a UseCase to a set of supporting Validations." ;
                  skos:prefLabel "Validation Policy"@en .


#################################################################
#    Individuals
#################################################################

###  https://rs.tdwg.org/bdqffdq/terms/MultiRecord
:MultiRecord rdf:type owl:NamedIndividual ,
                      :ResourceType ;
             rdfs:comment "A data set." ;
             rdfs:label "Multi Record"@en ;
             skos:definition "A set of one or more Single Records." ;
             skos:prefLabel "Multi Record" .


###  https://rs.tdwg.org/bdqffdq/terms/SingleRecord
:SingleRecord rdf:type owl:NamedIndividual ,
                       :ResourceType ;
              rdfs:comment "A record from a dataset.  May be a single row in a table, or rows related across several tables, or a graph of data.   Single in that it has one instance of a core concept from the perspective of information elements assessed for a UseCase.  For example, in a use case where occurences are central, a SingleRecord would represent a single occurrence, but could have multiple identifications and multiple taxa related to it in a graph or data structure.  However, in a UseCase where taxa are central, a SingleRecord would represent a single Taxon entity (and might have multiple occurrences related to it as part of the SingleRecord, so long as the graph was limited before reaching other Taxon entities)."@en ;
              rdfs:label "Single Record"@en ;
              skos:prefLabel "Single Record" .


#################################################################
#    General axioms
#################################################################

[ rdf:type owl:AllDisjointClasses ;
  owl:members ( :AbstractInformationElement
                :ActedUpon
                :Consulted
              )
] .


[ rdf:type owl:AllDisjointClasses ;
  owl:members ( :Amendment
                :Issue
                :Measure
                :Validation
              )
] .


###  Generated by the OWL API (version 4.5.29.2024-05-13T12:11:03Z) https://github.com/owlcs/owlapi
