@prefix : <https://rs.tdwg.org/bdqffdq/terms/> .
@prefix owl: <http://www.w3.org/2002/07/owl#> .
@prefix rdf: <http://www.w3.org/1999/02/22-rdf-syntax-ns#> .
@prefix xml: <http://www.w3.org/XML/1998/namespace> .
@prefix xsd: <http://www.w3.org/2001/XMLSchema#> .
@prefix rdfs: <http://www.w3.org/2000/01/rdf-schema#> .
@prefix skos: <http://www.w3.org/2004/02/skos/core#> .
@base <https://rs.tdwg.org/bdqffdq/terms> .

<https://rs.tdwg.org/bdqffdq/terms> rdf:type owl:Ontology ;
                                     rdfs:comment "The classes and object properties found in this ontology are dedicated to fundamental and derived concepts from the Fitness For Use Framework described in the paper by Veiga et al available at: http://journals.plos.org/plosone/article?id=10.1371/journal.pone.0178731" ;
                                     rdfs:label "Fittnes for Use Framework" .

#################################################################
#    Annotation properties
#################################################################

###  http://www.w3.org/2004/02/skos/core#definition
skos:definition rdf:type owl:AnnotationProperty .


###  http://www.w3.org/2004/02/skos/core#prefLabel
skos:prefLabel rdf:type owl:AnnotationProperty .


#################################################################
#    Object Properties
#################################################################

###  https://rs.tdwg.org/bdqffdq/terms#hasDataQualityDimension
:hasDataQualityDimension rdf:type owl:ObjectProperty ;
                         rdfs:label "has Data Quality Dimension"@en ;
                         skos:prefLabel "has Data Quality Dimension"@en .


###  https://rs.tdwg.org/bdqffdq/terms#hasPolicy
:hasPolicy rdf:type owl:ObjectProperty .


###  https://rs.tdwg.org/bdqffdq/terms#hasUseCase
:hasUseCase rdf:type owl:ObjectProperty .


###  https://rs.tdwg.org/bdqffdq/terms/amendmentProperties
:amendmentProperties rdf:type owl:ObjectProperty ;
                     rdfs:comment "Sub properties of this type group object properties that apply to amendment concepts such as AmendmentPolicy (DQ Needs), AmendmentMethod (DQ Solutions) and Amendment (DQ Reports)." .


###  https://rs.tdwg.org/bdqffdq/terms/composedOf
:composedOf rdf:type owl:ObjectProperty ;
            rdfs:range [ rdf:type owl:Restriction ;
                         owl:onProperty :hasSpecification ;
                         owl:someValuesFrom :InformationElement
                       ] ;
            rdfs:comment "Describes the properties from a controlled vocabulary that compose an InformationElement. For example, an InformationElement may be \"composedOf\" properties such as dwc:day, dwc:month and dwc:year." .


###  https://rs.tdwg.org/bdqffdq/terms/coversUseCase
:coversUseCase rdf:type owl:ObjectProperty ;
               rdfs:domain [ rdf:type owl:Restriction ;
                             owl:onProperty :hasInformationElement ;
                             owl:someValuesFrom :UseCase
                           ] ;
               rdfs:comment "Used by concepts in the DQ Needs category to describe the relationship between DQ Policies (ValidationPolicy, AmendmentPolicy, MeasurementPolicy) and an instance of the use case covered by that policy." .


###  https://rs.tdwg.org/bdqffdq/terms/dimensionInContext
:dimensionInContext rdf:type owl:ObjectProperty ;
                    rdfs:subPropertyOf :measurementProperties ;
                    rdfs:domain [ rdf:type owl:Restriction ;
                                  owl:onProperty :dimensionInContext ;
                                  owl:someValuesFrom :ContextualizedDimension
                                ] ;
                    rdfs:range [ rdf:type owl:Restriction ;
                                 owl:onProperty :dimensionInContext ;
                                 owl:someValuesFrom :MeasurementMethod
                               ] ,
                               [ rdf:type owl:Restriction ;
                                 owl:onProperty :dimensionInContext ;
                                 owl:someValuesFrom :MeasurementPolicy
                               ] ;
                    rdfs:comment "Describes the relationship between an Amendment concept in FFDQ (needs, solutions, reports) and a ContextualizedDimension." .


###  https://rs.tdwg.org/bdqffdq/terms/enhancementInContext
:enhancementInContext rdf:type owl:ObjectProperty ;
                      rdfs:subPropertyOf :amendmentProperties ;
                      rdfs:domain [ rdf:type owl:Restriction ;
                                    owl:onProperty :enhancementInContext ;
                                    owl:someValuesFrom :ContextualizedEnhancement
                                  ] ;
                      rdfs:range [ rdf:type owl:Restriction ;
                                   owl:onProperty :enhancementInContext ;
                                   owl:someValuesFrom :AmendmentMethod
                                 ] ,
                                 [ rdf:type owl:Restriction ;
                                   owl:onProperty :enhancementInContext ;
                                   owl:someValuesFrom :AmendmentPolicy
                                 ] ;
                      rdfs:comment "Describes the relationship between an Amendment concept in FFDQ (needs, solutions, reports) and a ContextualizedEnhancement." .


###  https://rs.tdwg.org/bdqffdq/terms/hasActedUponInformationElement
:hasActedUponInformationElement rdf:type owl:ObjectProperty ;
                                rdfs:subPropertyOf :hasInformationElement ;
                                rdfs:comment "Provides a relationship between FFDQ concepts and the information elements that are ActedUpon in a test."@en .


###  https://rs.tdwg.org/bdqffdq/terms/hasConsultedInformationElement
:hasConsultedInformationElement rdf:type owl:ObjectProperty ;
                                rdfs:subPropertyOf :hasInformationElement ;
                                rdfs:comment "Provides a relationship between FFDQ concepts and the information elements that are Consulted, but not ActedUpon in a test."@en .


###  https://rs.tdwg.org/bdqffdq/terms/hasDimension
:hasDimension rdf:type owl:ObjectProperty ;
              rdfs:subPropertyOf :measurementProperties ;
              rdfs:domain [ rdf:type owl:Restriction ;
                            owl:onProperty :hasDimension ;
                            owl:someValuesFrom :DataQualityDimension
                          ] ;
              rdfs:range [ rdf:type owl:Restriction ;
                           owl:onProperty :hasDimension ;
                           owl:someValuesFrom :ContextualizedDimension
                         ] ;
              rdfs:comment "Used to link the derived concept of a ContextualizedDimension to the fundamental concept of a Dimension." .


###  https://rs.tdwg.org/bdqffdq/terms/hasEnhancement
:hasEnhancement rdf:type owl:ObjectProperty ;
                rdfs:subPropertyOf :amendmentProperties ;
                rdfs:domain [ rdf:type owl:Restriction ;
                              owl:onProperty :hasEnhancement ;
                              owl:someValuesFrom :Amendmenent
                            ] ;
                rdfs:range [ rdf:type owl:Restriction ;
                             owl:onProperty :hasEnhancement ;
                             owl:someValuesFrom :ContextualizedEnhancement
                           ] ;
                rdfs:comment "Used to link the derived concept of a ContextualizedEnhancement to the fundamental concept of an Enhancement." .


###  https://rs.tdwg.org/bdqffdq/terms/hasInformationElement
:hasInformationElement rdf:type owl:ObjectProperty ;
                       rdfs:domain [ rdf:type owl:Restriction ;
                                     owl:onProperty :hasInformationElement ;
                                     owl:someValuesFrom :InformationElement
                                   ] ;
                       rdfs:comment "Provides a relationship between FFDQ concepts and the information elements. For example, ContextualizedCriterion uses this property along with hasResourceType to define a criterion in the context of related information elements." .


###  https://rs.tdwg.org/bdqffdq/terms/hasIssue
:hasIssue rdf:type owl:ObjectProperty ;
          rdfs:subPropertyOf :problemProperties ;
          rdfs:domain [ rdf:type owl:Restriction ;
                        owl:onProperty :hasIssue ;
                        owl:someValuesFrom :Issue
                      ] ;
          rdfs:range [ rdf:type owl:Restriction ;
                       owl:onProperty :hasIssue ;
                       owl:someValuesFrom :ContextualizedIssue
                     ] ;
          rdfs:comment "Used to link the derived concept of a ContextualizedIssue to the fundamental concept of a Problem." .


###  https://rs.tdwg.org/bdqffdq/terms/hasResourceType
:hasResourceType rdf:type owl:ObjectProperty ;
                 rdfs:comment "Provides additional metadata, along with the information elements, that describes the level (SingleRecord or MultiRecord) at which the FFDQ concept operates. For example, an enhancementInContext with resource type of MultiRecord could be used to define an Amendment that applies at the level of multiple record values." .


###  https://rs.tdwg.org/bdqffdq/terms/hasResponseResult
:hasResponseResult rdf:type owl:ObjectProperty ;
                   rdfs:subPropertyOf :reportProperties ;
                   rdfs:comment "Used in the DQ Report concept to describe response result objects. For example, values could be bdq:RUN_HAS_RESULT or bdq:INTERNAL_PREREQUISITES_NOT_MET.   If Response.results are not objects, use the datatype property hasResponseResultValue"@en .


###  https://rs.tdwg.org/bdqffdq/terms/hasResponseStatus
:hasResponseStatus rdf:type owl:ObjectProperty ;
                   rdfs:subPropertyOf :reportProperties ;
                   rdfs:comment "Used in the DQ Report concept to describe result status. For example, in the case of a Validation result, values could be bdq:COMPLIANT or bdq:NON_COMPLIANT." .


###  https://rs.tdwg.org/bdqffdq/terms/hasSpecification
:hasSpecification rdf:type owl:ObjectProperty ;
                  rdfs:domain [ rdf:type owl:Restriction ;
                                owl:onProperty :hasSpecification ;
                                owl:someValuesFrom :Specification
                              ] ;
                  rdfs:range [ rdf:type owl:Restriction ;
                               owl:onProperty :hasSpecification ;
                               owl:someValuesFrom :DataQualityNeed
                             ] ;
                  rdfs:comment "Describes the relationship between a derived FFDQ concept and the fundamental concept of a specification (technical description of a test)." .


###  https://rs.tdwg.org/bdqffdq/terms/hasStatus
:hasStatus rdf:type owl:ObjectProperty ;
           rdfs:comment "Used in the DQ Report concept to describe result status. For example, in the case of a Validation result, values could be COMPLIANT or NON_COMPLIANT." .


###  https://rs.tdwg.org/bdqffdq/terms/hasValidation
:hasValidation rdf:type owl:ObjectProperty ;
               rdfs:subPropertyOf :validationProperties ;
               rdfs:domain [ rdf:type owl:Restriction ;
                             owl:onProperty :hasValidation ;
                             owl:someValuesFrom :Validation
                           ] ;
               rdfs:range [ rdf:type owl:Restriction ;
                            owl:onProperty :hasValidation ;
                            owl:someValuesFrom :ContextualizedCriterion
                          ] ;
               rdfs:comment "Used to link the derived concept of a ContextualizedCriterion to the fundamental concept of a Criterion." .


###  https://rs.tdwg.org/bdqffdq/terms/implementedBy
:implementedBy rdf:type owl:ObjectProperty ;
               rdfs:domain [ rdf:type owl:Restriction ;
                             owl:onProperty :implementedBy ;
                             owl:someValuesFrom :Mechanism
                           ] ;
               rdfs:range [ rdf:type owl:Restriction ;
                            owl:onProperty :implementedBy ;
                            owl:someValuesFrom :Implementation
                          ] ;
               rdfs:comment "Describes the link between the Implementation concept in FFDQ and the Mechanism that implements some specification (also defined in Implementation)." .


###  https://rs.tdwg.org/bdqffdq/terms/improvedBy
:improvedBy rdf:type owl:ObjectProperty ;
            rdfs:domain [ rdf:type owl:Restriction ;
                          owl:onProperty :improvedBy ;
                          owl:someValuesFrom :ContextualizedEnhancement
                        ] ;
            rdfs:range [ rdf:type owl:Restriction ;
                         owl:onProperty :improvedBy ;
                         owl:someValuesFrom :ImprovementTarget
                       ] ;
            rdfs:comment "Object property that describes an enhancement, as part of the ImprovementTarget, that would improve data acted upon by some set of measures or validations.  This can be used to determine which measures and validations are improved upon by a given amendment." .


###  https://rs.tdwg.org/bdqffdq/terms/issueInContext
:issueInContext rdf:type owl:ObjectProperty ;
                rdfs:subPropertyOf :problemProperties ;
                rdfs:domain [ rdf:type owl:Restriction ;
                              owl:onProperty :issueInContext ;
                              owl:someValuesFrom :ContextualizedIssue
                            ] ;
                rdfs:range [ rdf:type owl:Restriction ;
                             owl:onProperty :issueInContext ;
                             owl:someValuesFrom :IssueMethod
                           ] ,
                           [ rdf:type owl:Restriction ;
                             owl:onProperty :issueInContext ;
                             owl:someValuesFrom :ProblemPolicy
                           ] ;
                rdfs:comment "Describes the relationship between a problem concept in FFDQ (needs, solutions, reports) and a ContextualizedIssue." .


###  https://rs.tdwg.org/bdqffdq/terms/measurementProperties
:measurementProperties rdf:type owl:ObjectProperty ;
                       rdfs:comment "Sub properties of this type group object properties that apply to measurement concepts such as MeasurementPolicy (DQ Needs), MeasurementMethod (DQ Solutions) and Measure (DQ Reports)." .


###  https://rs.tdwg.org/bdqffdq/terms/problemProperties
:problemProperties rdf:type owl:ObjectProperty ;
                   rdfs:comment "Sub properties of this type group object properties that apply to problem concepts such as ProblemPolicy (DQ Needs), ProblemMethod (DQ Solutions) and Issue (DQ Reports)." .


###  https://rs.tdwg.org/bdqffdq/terms/reportProperties
:reportProperties rdf:type owl:ObjectProperty .


###  https://rs.tdwg.org/bdqffdq/terms/targetedCriterion
:targetedCriterion rdf:type owl:ObjectProperty ;
                   rdfs:subPropertyOf owl:topObjectProperty ;
                   rdfs:domain [ rdf:type owl:Restriction ;
                                 owl:onProperty :targetedCriterion ;
                                 owl:someValuesFrom :ContextualizedCriterion
                               ] ;
                   rdfs:range [ rdf:type owl:Restriction ;
                                owl:onProperty :targetedCriterion ;
                                owl:someValuesFrom :ImprovementTarget
                              ] ;
                   rdfs:comment "The criteria targeted by some enhancement via the ImprovementTarget object." .


###  https://rs.tdwg.org/bdqffdq/terms/targetedDimension
:targetedDimension rdf:type owl:ObjectProperty ;
                   rdfs:domain [ rdf:type owl:Restriction ;
                                 owl:onProperty :targetedDimension ;
                                 owl:someValuesFrom :ContextualizedDimension
                               ] ;
                   rdfs:range [ rdf:type owl:Restriction ;
                                owl:onProperty :targetedDimension ;
                                owl:someValuesFrom :ImprovementTarget
                              ] ;
                   rdfs:comment "The dimension targeted by some enhancement via the ImprovementTarget object." .


###  https://rs.tdwg.org/bdqffdq/terms/targetedIssue
:targetedIssue rdf:type owl:ObjectProperty ;
               rdfs:domain [ rdf:type owl:Restriction ;
                             owl:onProperty :targetedIssue ;
                             owl:someValuesFrom :Issue
                           ] ;
               rdfs:range [ rdf:type owl:Restriction ;
                            owl:onProperty :targetedIssue ;
                            owl:someValuesFrom :ImprovementTarget
                          ] ;
               rdfs:comment "The issue targeted by some problem via the ImprovementTarget object." .


###  https://rs.tdwg.org/bdqffdq/terms/validationInContext
:validationInContext rdf:type owl:ObjectProperty ;
                     rdfs:subPropertyOf :validationProperties ;
                     rdfs:domain [ rdf:type owl:Restriction ;
                                   owl:onProperty :validationInContext ;
                                   owl:someValuesFrom :ContextualizedCriterion
                                 ] ;
                     rdfs:range [ rdf:type owl:Restriction ;
                                  owl:onProperty :validationInContext ;
                                  owl:someValuesFrom :ValidationMethod
                                ] ,
                                [ rdf:type owl:Restriction ;
                                  owl:onProperty :validationInContext ;
                                  owl:someValuesFrom :ValidationPolicy
                                ] ;
                     rdfs:comment "Describes the relationship between a validation concept in FFDQ (needs, solutions, reports) and a contextualizedCriterion." .


###  https://rs.tdwg.org/bdqffdq/terms/validationProperties
:validationProperties rdf:type owl:ObjectProperty ;
                      rdfs:comment "Sub properties of this type group object properties that apply to validation concepts such as ValidationPolicy (DQ Needs), ValidationMethod (DQ Solutions) and Validation (DQ Reports)." .


#################################################################
#    Data properties
#################################################################

###  https://rs.tdwg.org/bdqffdq/terms#hasCriterion
:hasCriterion rdf:type owl:DatatypeProperty .


###  https://rs.tdwg.org/bdqffdq/terms#hasEnhancement
:hasEnhancement rdf:type owl:DatatypeProperty .


###  https://rs.tdwg.org/bdqffdq/terms/hasAuthoritiesDefaults
:hasAuthoritiesDefaults rdf:type owl:DatatypeProperty ;
                        rdfs:range xsd:string ;
                        rdfs:comment "Details of the bdq:sourceAuthoritiy listed in a Specification, along with Parameters that may be provided to the expected response along with their default values." ;
                        rdfs:label "has Authorities and Defaults"@en ;
                        skos:prefLabel "has Authorities and Defaults" .


###  https://rs.tdwg.org/bdqffdq/terms/hasExpectedResponse
:hasExpectedResponse rdf:type owl:DatatypeProperty ;
                     rdfs:range xsd:string ;
                     rdfs:comment "The description of the logic of a test specification.  An expected response is expected to be a data property of a Specification"@en ;
                     rdfs:label "has Expected Response"@en ;
                     skos:prefLabel "has Expected Response"@en .


###  https://rs.tdwg.org/bdqffdq/terms/hasResponseResultValue
:hasResponseResultValue rdf:type owl:DatatypeProperty ;
                        rdfs:range xsd:double ;
                        rdfs:label "has response result value" ;
                        skos:prefLabel "has response result value" .


#################################################################
#    Classes
#################################################################

###  https://rs.tdwg.org/bdqffdq/terms#AbstractInformationElement
:AbstractInformationElement rdf:type owl:Class ;
                            rdfs:subClassOf :InformationElement .


###  https://rs.tdwg.org/bdqffdq/terms/ActedUpon
:ActedUpon rdf:type owl:Class ;
           rdfs:subClassOf :InformationElement ;
           rdfs:comment "An information element to which a Result applies."@en ;
           rdfs:label "Acted Upon"@en .


###  https://rs.tdwg.org/bdqffdq/terms/Amendmenent
:Amendmenent rdf:type owl:Class ;
             rdfs:subClassOf :AmendmentConcept ,
                             :DataQualityNeed ;
             rdfs:comment "Describes a proposal for enhancement of original data, which if accepted, would improve the quality of the data for some use. For example, \"Recommends valid value for taxon name in a single record\".  Amendments may describe proposed changes to data values, or to processes for the production and manipulation of data, for example an Amendment on a SingleRecord may provide criteria for proposing that latitude and longitude are transposed in that record, or a similar Amendment on a MultiRecord may provide critera for proposing that all latitudes and longitudes from some data source have been transposed, and the mapping of data values to transport terms should be changed.  An Amendment is the data quality needs concept that paralells an AmendmentMethod at the solutions level, and an AmmendmentAssertion at the report level."@en ;
             rdfs:label "Amendment"@en ;
             skos:prefLabel "Amendment"@en .


###  https://rs.tdwg.org/bdqffdq/terms/AmendmentAssertion
:AmendmentAssertion rdf:type owl:Class ;
                    rdfs:subClassOf :AmendmentConcept ,
                                    :Assertion ;
                    rdfs:comment "The Amendment assertion type is a report level concept that describes a run of a test that proposes changes based on some data quality enhancement. The Amendment concept in FFDQ consists of a run result that includes a status (FILLED_IN, TRANSPOSED, etc) as well as the proposed changes to values from the original data." ;
                    rdfs:label "Amendment Assertion"@en ;
                    skos:prefLabel "Amendment Assertion"@en .


###  https://rs.tdwg.org/bdqffdq/terms/AmendmentConcept
:AmendmentConcept rdf:type owl:Class ;
                  rdfs:label "Amendment Concept"@en ;
                  skos:definition "A term involved in proposals of changes to data or process to improve data quallity to fit expressed data quality needs."@en ;
                  skos:prefLabel "Amendment Concept"@en .


###  https://rs.tdwg.org/bdqffdq/terms/AmendmentMethod
:AmendmentMethod rdf:type owl:Class ;
                 rdfs:subClassOf :AmendmentConcept ,
                                 :DataQualityMethod ;
                 rdfs:comment "The AmendmentMethod in FFDQ is a DQ Solutions level concept describing the relationship between a specification (technical description of a test) and an enhancement in the context of resource type (SingleRecord or MultiRecord) and associated information elements." ;
                 rdfs:label "Amendment Method"@en ;
                 skos:prefLabel "Amendment Method"@en .


###  https://rs.tdwg.org/bdqffdq/terms/AmendmentPolicy
:AmendmentPolicy rdf:type owl:Class ;
                 rdfs:subClassOf :AmendmentConcept ,
                                 :NeedConcept ;
                 rdfs:comment "A Data Quality needs level concept that describes how some bdqffdq:contextualizedEnhancement relates to a bdqffdq:UseCase. This relationship defines which amendments are supported by a given use case." ;
                 rdfs:label "Amendment Policy"@en ;
                 skos:definition "The set of Contextualized Enhancements that support a Use Case."@en ;
                 skos:prefLabel "Amendment Policy"@en .


###  https://rs.tdwg.org/bdqffdq/terms/Assertion
:Assertion rdf:type owl:Class ;
           rdfs:subClassOf :ReportConcept ;
           rdfs:comment """The Assertion type in FFDQ is the fundamental concept that makes up a data quality report. Assertion can be any one of four types (represented as subClasses), Measure, Validation, Issue, and Amendement.

The assertion concept consists of a specification (the technical description of a performed test), a data resource (initial values of input data expressed in terms of some controlled vocabulary), the mechanism (external service, actor, or code that performs the test), and some form of result.""" ;
           rdfs:label "Assertion"@en ;
           skos:prefLabel "Assertion"@en .


###  https://rs.tdwg.org/bdqffdq/terms/Consulted
:Consulted rdf:type owl:Class ;
           rdfs:subClassOf :InformationElement ;
           rdfs:comment "An Information Element the content of which is examined to assert a result on one or more other Information Elements"@en ;
           rdfs:label "Consulted"@en .


###  https://rs.tdwg.org/bdqffdq/terms/ContextualizedCriterion
:ContextualizedCriterion rdf:type owl:Class ;
                         rdfs:subClassOf :DataQualityNeed ,
                                         :ValidationConcept ;
                         rdfs:comment "Describes an instance of the criterion concept in terms of the associated information elements from some controlled vocabulary (fields actedUpon or consulted), and a resource type of SingleRecord or MultiRecord." ;
                         skos:prefLabel "Contextualized Criterion"@en .


###  https://rs.tdwg.org/bdqffdq/terms/ContextualizedDimension
:ContextualizedDimension rdf:type owl:Class ;
                         rdfs:subClassOf :DataQualityNeed ,
                                         :MeaurementConcept ;
                         rdfs:comment "Describes an instance of the measure concept in terms of the associated information elements from some controlled vocabulary (fields actedUpon or consulted), and a resource type of SingleRecord or MultiRecord." ;
                         rdfs:label "Contextualized Dimension"@en ;
                         skos:prefLabel "Contextualized Dimension"@en .


###  https://rs.tdwg.org/bdqffdq/terms/ContextualizedEnhancement
:ContextualizedEnhancement rdf:type owl:Class ;
                           rdfs:subClassOf :AmendmentConcept ,
                                           :DataQualityNeed ;
                           rdfs:comment "Describes an instance of the enhancement concept in terms of the associated information elements from some controlled vocabulary (fields actedUpon or consulted), and a resource type of SingleRecord or MultiRecord." ;
                           rdfs:label "Contextualized Enhancement"@en ;
                           skos:prefLabel "Contextualized Enhancement"@en .


###  https://rs.tdwg.org/bdqffdq/terms/ContextualizedIssue
:ContextualizedIssue rdf:type owl:Class ;
                     rdfs:subClassOf :DataQualityNeed ,
                                     :IssueConcept ;
                     rdfs:comment "Describes an instance of the issue concept in terms of the associated information elements from some controlled vocabulary (fields actedUpon or consulted), and a resource type of SingleRecord or MultiRecord." ;
                     rdfs:label "Contextualized Issue"@en ;
                     skos:prefLabel "Contextualized Issue"@en .


###  https://rs.tdwg.org/bdqffdq/terms/DataQualityDimension
:DataQualityDimension rdf:type owl:Class ;
                      rdfs:comment "Describes the aspect of data quality (accuracy, precision, completeness, etc.) that a test examines. For example, \"precision\" in \"coordinate precision of single records\"."@en ;
                      rdfs:label "Data Quality Dimension"@en ;
                      skos:definition "An aspect of data quality."@en ;
                      skos:prefLabel "Data Quality Dimension" .


###  https://rs.tdwg.org/bdqffdq/terms/DataQualityMethod
:DataQualityMethod rdf:type owl:Class ;
                   rdfs:subClassOf :SolutionsConcept ;
                   rdfs:label "Data Quality Method"@en ;
                   skos:prefLabel "Data Quality Method"@en .


###  https://rs.tdwg.org/bdqffdq/terms/DataQualityNeed
:DataQualityNeed rdf:type owl:Class ;
                 rdfs:subClassOf :NeedConcept ;
                 rdfs:label "Data Quality Need"@en ;
                 skos:prefLabel "Data Quality Need"@en .


###  https://rs.tdwg.org/bdqffdq/terms/DataQualityReport
:DataQualityReport rdf:type owl:Class ;
                   rdfs:subClassOf :ReportConcept ;
                   rdfs:comment "The FFDQ Report concept consists of a set of assertions (measures, validations and amendments) that represent the output of a workflow/actor run.  These assertions form an account of the fitness for use of a tested data set for a specified use, as produced by a Mechanism."@en ;
                   rdfs:label "Data Quality Report"@en ;
                   skos:prefLabel "Data Quality Report"@en .


###  https://rs.tdwg.org/bdqffdq/terms/DataResource
:DataResource rdf:type owl:Class ;
              rdfs:subClassOf :ReportConcept ;
              rdfs:comment "Describes a data resource described in terms of a controlled vocabulary such as dwc and represents the original values of the data operated on by an assertion test (i.e. an instance of dwc:Occurrence)." ;
              rdfs:label "Data Resource"@en ;
              skos:prefLabel "Data Resource"@en .


###  https://rs.tdwg.org/bdqffdq/terms/Implementation
:Implementation rdf:type owl:Class ;
                rdfs:subClassOf :SolutionsConcept ;
                rdfs:comment "The FFDQ derived concept of an Implementation describes the relationship between a specification (technical description of a test) and the mechanism that implements it." ;
                rdfs:label "Implementation"@en ;
                skos:prefLabel "Implementation"@en .


###  https://rs.tdwg.org/bdqffdq/terms/ImprovementTarget
:ImprovementTarget rdf:type owl:Class ;
                   rdfs:subClassOf :NeedConcept ;
                   rdfs:comment "The ImprovementTarget concept in FFDQ describes which measures and validations are improved by some amendment. ImprovementTarget includes relationships between a contextualizedEnhancement (for an Amendment) and one or more contextualizedCriterion (link to validations) or contextualizedDimensions (link to measures)." ;
                   rdfs:label "Improvement Target"@en ;
                   skos:prefLabel "Improvement Target"@en .


###  https://rs.tdwg.org/bdqffdq/terms/InformationElement
:InformationElement rdf:type owl:Class ;
                    rdfs:comment "An information element identifies a portion of data to which a test pertains.  The information element in FFDQ can be represented as a single or composite element that consists of one or more terms from a controlled vocabulary (fields actedUpon or consulted by an assertion test) that identifies concepts in data relevant to a use case.  An abstraction or a concrete term that represents relevant content (e.g., coordinates; dwc.decimalLatitude, dwc:decimalLongitude)."@en ;
                    rdfs:label "Information Element"@en ;
                    skos:prefLabel "Information Element"@en .


###  https://rs.tdwg.org/bdqffdq/terms/Issue
:Issue rdf:type owl:Class ;
       rdfs:subClassOf :DataQualityNeed ,
                       :IssueConcept ;
       rdfs:comment "Describes criteria by which data which lack quality for some purpose may be identified.  An issue is phrased in a negative sense, and approximantes an inverse of a Validation.  An Issue identifies data that lack or may lack quality.  An Issue may flag a POSSIBLE_PROBLEM that would need further review to determine if the data have qulity for some purpose,  If the conditions described by an issue are identified by a test, the Problem Assertion result will be either HAS_PROBLEM or POSSIBLE_PROBLEM, if no issue is found with the data the result will be NO_PROBLEM.  NO_PROBLEM, unlike COMPLIANT for a Validation, does not assert that data are fit for some purpose.    An Issue is the data quality needs concept that paralells a IssueMethod at the solutions level, and a IssieAssertion at the report level."@en ;
       rdfs:label "Issue"@en ;
       skos:prefLabel "Issue"@en .


###  https://rs.tdwg.org/bdqffdq/terms/IssueAssertion
:IssueAssertion rdf:type owl:Class ;
                rdfs:subClassOf :Assertion ,
                                :IssueConcept ;
                rdfs:comment "The DQ report concept describing a test for the negative case. If a problem was found the result has a status of HAS_PROBLEM otherwise the status is NO_PROBLEM." ;
                rdfs:label "Issue Assertion"@en ;
                skos:prefLabel "Issue Assertion"@en .


###  https://rs.tdwg.org/bdqffdq/terms/IssueConcept
:IssueConcept rdf:type owl:Class ;
              rdfs:comment "Issue terms are expressed in a negative sense, they identify data that do not or may not conform to quality needs."@en ;
              rdfs:label "Issue Concept"@en ;
              skos:definition "A term involved in flagging problems or potential problems in assessment of data quality that would or might prevent the data from meeting expressed data quality needs.."@en ;
              skos:prefLabel "Issue Concept"@en .


###  https://rs.tdwg.org/bdqffdq/terms/IssueMethod
:IssueMethod rdf:type owl:Class ;
             rdfs:subClassOf :DataQualityMethod ,
                             :IssueConcept ;
             rdfs:comment "The ProblemMethod in FFDQ is a DQ Solutions level concept describing the relationship between a specification (technical description of a test) and an issue in the context of resource type (SingleRecord or MultiRecord) and associated information elements." ;
             rdfs:label "Issue Method"@en ;
             skos:prefLabel "Issue Method"@en .


###  https://rs.tdwg.org/bdqffdq/terms/Measure
:Measure rdf:type owl:Class ;
         rdfs:subClassOf :DataQualityNeed ,
                         :MeaurementConcept ;
         rdfs:comment "Describes the criteria for measuring an aspect of data quality related to some data quality need.   May be criteria for determining that data are COMPLETE or NOT_COMPLETE, or may be criteria for asserting a numeric measurement.  COMPLETE or NOT_COMPLETE measures are fundamental to data quality control, as set of data are filtered to the subset of data have quality for some need if all records are COMPLETE for all pertenent Measures.  A Measure is the data quality needs concept that paralells a MeasurementMethod at the solutions level, and a MeasurementAssertion at the report level."@en ;
         rdfs:label "Measure"@en ;
         skos:prefLabel "Measure"@en .


###  https://rs.tdwg.org/bdqffdq/terms/MeasurementAssertion
:MeasurementAssertion rdf:type owl:Class ;
                      rdfs:subClassOf :Assertion ,
                                      :MeaurementConcept ;
                      rdfs:comment "The Measure assertion type is a report level concept that describes a run of a test that performs a measurement according to some data quality dimension. In FFDQ, the Measure concept consists of a run result of COMPLETE or NOT_COMPLETE or a value of the measurement (i.e. a measure of dwc:eventDate duration in seconds)." ;
                      rdfs:label "Measurement Assertion"@en ;
                      skos:prefLabel "Measurement Assertion"@en .


###  https://rs.tdwg.org/bdqffdq/terms/MeasurementMethod
:MeasurementMethod rdf:type owl:Class ;
                   rdfs:subClassOf :DataQualityMethod ,
                                   :MeaurementConcept ;
                   rdfs:comment "The MeasurementMethod in FFDQ is a DQ Solutions level concept describing the relationship between a specification (technical description of a test) and a dimension in the context of resource type (SingleRecord or MultiRecord) and associated information elements." ;
                   rdfs:label "Measurement Method"@en ;
                   skos:prefLabel "Measurement Method"@en .


###  https://rs.tdwg.org/bdqffdq/terms/MeasurementPolicy
:MeasurementPolicy rdf:type owl:Class ;
                   rdfs:subClassOf :MeaurementConcept ,
                                   :NeedConcept ;
                   rdfs:comment "The MeasurementPolicy in FFDQ is a DQ Needs level concept that describes how some contextualizedDimension relates to a use case. This relationship defines which measures are supported by a given use case." ;
                   rdfs:label "Measurement Policy"@en ;
                   skos:prefLabel "Measurement Policy"@en .


###  https://rs.tdwg.org/bdqffdq/terms/MeaurementConcept
:MeaurementConcept rdf:type owl:Class ;
                   rdfs:label "Measurement Concept"@en ;
                   skos:definition "A term involved in measurement of data quality with regards to expressed data quality needs."@en ;
                   skos:prefLabel "Measurement Concept"@en .


###  https://rs.tdwg.org/bdqffdq/terms/Mechanism
:Mechanism rdf:type owl:Class ;
           rdfs:subClassOf :SolutionsConcept ;
           rdfs:comment "The FFDQ concept of mechanism describes the entity that performs an assertion test (code, external service, actor, etc.). Tied to a specification via the concept of an Implementation." ;
           rdfs:label "Mechanism"@en ;
           skos:prefLabel "Mechanism"@en .


###  https://rs.tdwg.org/bdqffdq/terms/NeedConcept
:NeedConcept rdf:type owl:Class ;
             rdfs:label "Need Concept"@en ;
             skos:definition "Category of concepts forming the Needs layer of the fittness for use framework."@en ;
             skos:prefLabel "Need Concept"@en .


###  https://rs.tdwg.org/bdqffdq/terms/Parameter
:Parameter rdf:type owl:Class ;
           rdfs:label "Parameter"@en ;
           skos:prefLabel "Parameter"@en .


###  https://rs.tdwg.org/bdqffdq/terms/ProblemPolicy
:ProblemPolicy rdf:type owl:Class ;
               rdfs:subClassOf :IssueConcept ,
                               :NeedConcept ;
               rdfs:comment "The ProblemPolicy in FFDQ is a DQ Needs level concept that describes how some contextualizedIssue relates to a use case. This relationship defines which problems are supported by a given use case." ;
               rdfs:label "Problem Policy"@en ;
               skos:prefLabel "Problem Policy"@en .


###  https://rs.tdwg.org/bdqffdq/terms/Profile
:Profile rdf:type owl:Class ;
         rdfs:subClassOf :NeedConcept ;
         rdfs:comment "Profile in FFDQ is a DQ Needs level concept describing the UseCases that make up some data quality operation such as the behavior of a single actor or workflow producing the relevant assertions." ;
         rdfs:label "Profile"@en ;
         skos:prefLabel "Profile"@en .


###  https://rs.tdwg.org/bdqffdq/terms/ReportConcept
:ReportConcept rdf:type owl:Class ;
               skos:definition "Category of concepts forming the Report layer of the fittness for use framework."@en ;
               skos:prefLabel "Report Concept"@en .


###  https://rs.tdwg.org/bdqffdq/terms/ResourceType
:ResourceType rdf:type owl:Class ;
              rdfs:comment "In bdqffdq the concept of ResourceType has instances for SingleRecord or MultiRecord" ;
              rdfs:label "Resource Type"@en ;
              skos:prefLabel "Resource Type"@en .


###  https://rs.tdwg.org/bdqffdq/terms/Result
:Result rdf:type owl:Class ;
        rdfs:subClassOf :ReportConcept ;
        rdfs:comment "The report result concept in FFDQ is represented as a value or a status for measures, just a result status for validations and a result status as well as values for changes propsed by amendments." ;
        rdfs:label "Response.result"@en ;
        skos:prefLabel "Response.result"@en .


###  https://rs.tdwg.org/bdqffdq/terms/ResultStatus
:ResultStatus rdf:type owl:Class ;
              rdfs:subClassOf :ReportConcept ;
              rdfs:comment """Depending on the assertion type would have values of COMPLIANT or NON_COMPLIANT for a Validation, COMPLETE or NOT_COMPLETE for a Measure, CURATED, FILLED_IN,TRANSPOSED, NO_CHANGE for an Amendment and HAS_PROBLEM NO_PROBLEM for a Problem.

A separate concept describes the result state as values of AMBIGIOUS, INTERNAL_PREREQUISITES_NOT_MET and EXTERNAL_PREREQUISITES_NOT_MET.""" ;
              rdfs:label "Response.status"@en ;
              skos:prefLabel "Response.status"@en .


###  https://rs.tdwg.org/bdqffdq/terms/SolutionsConcept
:SolutionsConcept rdf:type owl:Class ;
                  rdfs:label "Solutions Concept"@en ;
                  skos:definition "Category of concepts forming the Solutions layer of the fittness for use framework."@en ;
                  skos:prefLabel "Solutions Concept"@en .


###  https://rs.tdwg.org/bdqffdq/terms/Specification
:Specification rdf:type owl:Class ;
               rdfs:subClassOf :NeedConcept ;
               rdfs:comment """A specification is a technical desription of an assertion test.

A specification is expected to have the following properies: 

Expected Response

Authorities and Parameters"""@en ;
               rdfs:label "Specification"@en ;
               skos:prefLabel "Specification"@en .


###  https://rs.tdwg.org/bdqffdq/terms/UseCase
:UseCase rdf:type owl:Class ;
         rdfs:subClassOf :NeedConcept ;
         rdfs:comment """The UseCase concept in FFDQ describes some data quality control use case. The Amendment, Measurement and Validation policies that make up a use case define which assertions cover a given use case.

An example of a UseCase could be \"Check for internal consistency of dates\", with validation policies for checking consistency between atomic date fields and an Amendment such as \"eventDate filled in from verbatim\".

Use Cases in bdqffdq are not the same as Use Cases in the software engineering sense, but  are similar bdqffdq formal statements derived from analyis of user stories.""" ;
         rdfs:label "Use Case"@en ;
         skos:prefLabel "Use Case"@en .


###  https://rs.tdwg.org/bdqffdq/terms/Validation
:Validation rdf:type owl:Class ;
            rdfs:subClassOf :DataQualityNeed ,
                            :ValidationConcept ;
            rdfs:comment "Describes the criteria for determining compliance of data to fill some data quality need.  Validations are phrased in a positive sense, they identify data which has quality for some need.  For example, \"The value of basisOfRecord of single records must be in the controlled vocabulary\".   A Validation is the data quality needs concept that paralells a ValidationMethod at the solutions level, and a ValidationAssertion at the report level.  ValidationAssertions may specify a result that is COMPLIANT, where the data has quality, or NOT_COMPLIANT, where the data lacks quality."@en ;
            rdfs:label "Validation"@en ;
            skos:prefLabel "Validation"@en .


###  https://rs.tdwg.org/bdqffdq/terms/ValidationAssertion
:ValidationAssertion rdf:type owl:Class ;
                     rdfs:subClassOf :Assertion ,
                                     :ValidationConcept ;
                     rdfs:comment "The Validation assertion type is a report level concept that describes a run of a test for validity. The Validation concept in FFDQ consists of a run result of COMPLIANT or NON_COMPLIANT and a criterion that describes the conditions for validity that result in a status of COMPLIANT." ;
                     rdfs:label "Vailidation Assertion"@en ;
                     skos:prefLabel "Vailidation Assertion"@en .


###  https://rs.tdwg.org/bdqffdq/terms/ValidationConcept
:ValidationConcept rdf:type owl:Class ;
                   rdfs:comment "Validation terms are expressed in a positive sense, they identify data that conform to needs."@en ;
                   rdfs:label "Validation Concept"@en ;
                   skos:definition "A term involved in statements about the conformance of data to expressed quality needs."@en ;
                   skos:prefLabel "Validation Concept"@en .


###  https://rs.tdwg.org/bdqffdq/terms/ValidationMethod
:ValidationMethod rdf:type owl:Class ;
                  rdfs:subClassOf :DataQualityMethod ,
                                  :ValidationConcept ;
                  rdfs:comment "The ValidationMethod in FFDQ is a DQ Solutions level concept describing the relationship between a specification (technical description of a test) and a criterion in the context of resource type (SingleRecord or MultiRecord) and associated information elements." ;
                  rdfs:label "Validation Method"@en ;
                  skos:prefLabel "Validation Method"@en .


###  https://rs.tdwg.org/bdqffdq/terms/ValidationPolicy
:ValidationPolicy rdf:type owl:Class ;
                  rdfs:subClassOf :NeedConcept ,
                                  :ValidationConcept ;
                  rdfs:comment "The ValidationPolicy in FFDQ is a DQ Needs level concept that describes how some contextualizedCriterion relates to a use case. This relationship defines which validations are supported by a given use case." ;
                  rdfs:label "Validation Policy"@en ;
                  skos:prefLabel "Validation Policy"@en .


#################################################################
#    Individuals
#################################################################

###  https://rs.tdwg.org/bdqffdq/terms/MultiRecord
:MultiRecord rdf:type owl:NamedIndividual ,
                      :ResourceType ;
             rdfs:label "Multi Record"@en .


###  https://rs.tdwg.org/bdqffdq/terms/SingleRecord
:SingleRecord rdf:type owl:NamedIndividual ,
                       :ResourceType ;
              rdfs:comment "A record from a dataset without dependencies on any other record."@en ;
              rdfs:label "Single Record"@en .


#################################################################
#    General axioms
#################################################################

[ rdf:type owl:AllDisjointClasses ;
  owl:members ( :AbstractInformationElement
                :ActedUpon
                :Consulted
              )
] .


[ rdf:type owl:AllDisjointClasses ;
  owl:members ( :Amendmenent
                :Issue
                :Measure
                :Validation
              )
] .


###  Generated by the OWL API (version 4.5.9.2019-02-01T07:24:44Z) https://github.com/owlcs/owlapi
